verified/subdir.mk
@@ -1,6 +1,6 @@
 DAFNYFLAGS = /autoTriggers:1 /noNLarith /timeLimit:30 /trace
 # NB: include paths are relative to the (generated) dfy file, not the CWD
-SPARTAN_INCLUDES = -i ARMspartan.dfy -i ARMprint.dfy $(SHA256_INCLUDES)
+SPARTAN_INCLUDES = -i ARMspartan.dfy -i ARMprint.dfy #$(SHA256_INCLUDES)
 SHA256_INCLUDES = -i sha_common.s.dfy -i sha256.s.dfy -i sha256.i.dfy 
 SPARTAN_DEPS = $(dir)/ARMdef.dll $(dir)/ARMprint.dll $(dir)/ARMspartan.dll $(dir)/sha256.s.dll
 
